

基态波函数

基态 $|\Omega\rangle$ 是 α 准粒子的真空态, 满足:

$$\alpha_i |\Omega\rangle = 0 \quad (1)$$

也即

$$\sum_{j=1}^N \left(w_{ji}^* a_j + v_{ji}^* a_j^\dagger \right) |\Omega\rangle = 0 \quad (2)$$

基态形式

$$|\Omega\rangle = \mathcal{N} \exp \left(\frac{1}{2} \sum_{i,j} f_{i,j} a_i^\dagger a_j^\dagger \right) |0_a\rangle \quad (3)$$

其中 $|0_a\rangle$ 是 a 费米子真空态, $f_{i,j} = -f_{j,i}$

由于

$$\left[a_i^\dagger a_j^\dagger, a_k^\dagger a_l^\dagger \right] = 0 \quad (4)$$

而

$$[A, B] = 0 \implies \exp(A + B) = \exp(A) \exp(B) \quad (5)$$

于是

$$\begin{aligned} |\Omega\rangle &= \mathcal{N} \exp \left(\frac{1}{2} \sum_{i,j} f_{i,j} a_i^\dagger a_j^\dagger \right) |0_a\rangle \\ &= \mathcal{N} \prod_{i,j} \exp \left(\frac{1}{2} f_{i,j} a_i^\dagger a_j^\dagger \right) |0_a\rangle \end{aligned} \quad (6)$$

注意到

$$\begin{aligned} \exp \left(\frac{1}{2} f_{i,j} a_i^\dagger a_j^\dagger \right) |0_a\rangle &= \sum_{k=0}^{\infty} \frac{1}{k!} \left(\frac{1}{2} f_{i,j} a_i^\dagger a_j^\dagger \right)^k |0_a\rangle \\ &= \left(1 + \frac{1}{1!} \cdot \frac{1}{2!} f_{i,j} a_i^\dagger a_j^\dagger + \frac{1}{2!} \cdot \frac{1}{2^2} a_i^\dagger a_j^\dagger a_i^\dagger a_j^\dagger + \dots \right) |0_a\rangle \\ &= \left(1 + \frac{1}{2} f_{i,j} a_i^\dagger a_j^\dagger \right) |0_a\rangle \end{aligned} \quad (7)$$

于是

$$\begin{aligned} |\Omega\rangle &= \mathcal{N} \prod_{i,j} \exp \left(\frac{1}{2} f_{i,j} a_i^\dagger a_j^\dagger \right) |0_a\rangle \\ &= \mathcal{N} \prod_{i,j} \left(1 + \frac{1}{2} f_{i,j} a_i^\dagger a_j^\dagger \right) |0_a\rangle \end{aligned} \quad (8)$$

求基态波函数 $f_{i,j}$

$$\alpha_i = \sum_{j=1}^N \left(w_{ji}^* a_j + v_{ji}^* a_j^\dagger \right)$$

$$|\Omega\rangle = \mathcal{N} \prod_{l,m} \left(1 + \frac{1}{2} f_{l,m} a_l^\dagger a_m^\dagger \right) |0_a\rangle \quad (9)$$

基态由

$$\alpha_i |\Omega\rangle = 0 \quad (10)$$

确定。

利用

$$AB = [A, B] + BA \quad (11)$$

$$\left[A, \prod_i B_i \right] = \sum_k \left(\prod_{j < k} B_j \right) [A, B_k] \left(\prod_{j > k} B_j \right) \quad (12)$$

$$\left[1 + \frac{1}{2} f_{i,j} a_i^\dagger a_j^\dagger, 1 + \frac{1}{2} f_{l,m} a_l^\dagger a_m^\dagger \right] = 0 \quad (13)$$

$$\begin{aligned} \left[a_j, 1 + \frac{1}{2} f_{l',m'} a_{l'}^\dagger a_{m'}^\dagger \right] &= \frac{1}{2} f_{l',m'} \left[a_j, a_{l'}^\dagger a_{m'}^\dagger \right] \\ &= \frac{1}{2} f_{l',m'} \left(\left[a_j, a_{l'}^\dagger \right] a_{m'}^\dagger + a_{l'}^\dagger \left[a_j, a_{m'}^\dagger \right] \right) \\ &= \frac{1}{2} f_{l',m'} \left[\left(\left\{ a_j, a_{l'}^\dagger \right\} - 2 a_{l'}^\dagger a_j \right) a_{m'}^\dagger + a_{l'}^\dagger \left(\left\{ a_j, a_{m'}^\dagger \right\} - 2 a_{m'}^\dagger a_j \right) \right] \\ &= \frac{1}{2} f_{l',m'} \left[\left(\delta_{j,l'} - 2 a_{l'}^\dagger a_j \right) a_{m'}^\dagger + a_{l'}^\dagger \left(\delta_{j,m'} - 2 a_{m'}^\dagger a_j \right) \right] \\ &= \frac{1}{2} f_{l',m'} \left(\delta_{j,l'} a_{m'}^\dagger + \delta_{j,m'} a_{l'}^\dagger - 2 a_{l'}^\dagger a_j a_{m'}^\dagger - 2 a_{l'}^\dagger a_{m'}^\dagger a_j \right) \\ &= \frac{1}{2} f_{l',m'} \left[\delta_{j,l'} a_{m'}^\dagger + \delta_{j,m'} a_{l'}^\dagger - 2 a_{l'}^\dagger \left(\delta_{j,m'} - a_{m'}^\dagger a_j \right) - 2 a_{l'}^\dagger a_{m'}^\dagger a_j \right] \\ &= \frac{1}{2} f_{l',m'} \left(\delta_{j,l'} a_{m'}^\dagger - \delta_{j,m'} a_{l'}^\dagger \right) \end{aligned} \quad (14)$$

$$\left[a_{m'}^\dagger, 1 + \frac{1}{2} f_{l,m} a_l^\dagger a_m^\dagger \right] = 0 \quad (15)$$

$$\begin{aligned} &\frac{1}{2} f_{l',m'} \left(\delta_{j,l'} a_{m'}^\dagger - \delta_{j,m'} a_{l'}^\dagger \right) \cdot \left(1 + \frac{1}{2} f_{l',m'} a_{l'}^\dagger a_{m'}^\dagger \right) \\ &= \frac{1}{2} f_{l',m'} \left(\delta_{j,l'} a_{m'}^\dagger - \delta_{j,m'} a_{l'}^\dagger \right) + \frac{1}{4} f_{l',m'}^2 \left(\delta_{j,l'} a_{m'}^\dagger - \delta_{j,m'} a_{l'}^\dagger \right) a_{l'}^\dagger a_{m'}^\dagger \\ &= \frac{1}{2} f_{l',m'} \left(\delta_{j,l'} a_{m'}^\dagger - \delta_{j,m'} a_{l'}^\dagger \right) \end{aligned} \quad (16)$$

有

$$\begin{aligned}
a_j \prod_{l,m} \left(1 + \frac{1}{2} f_{l,m} a_l^\dagger a_m^\dagger \right) |0_a\rangle &= \left[a_j, \prod_{l,m} \left(1 + \frac{1}{2} f_{l,m} a_l^\dagger a_m^\dagger \right) \right] |0_a\rangle + \prod_{l,m} \left(1 + \frac{1}{2} f_{l,m} a_l^\dagger a_m^\dagger \right) a_j |0_a\rangle \\
&= \left[a_j, \prod_{l,m} \left(1 + \frac{1}{2} f_{l,m} a_l^\dagger a_m^\dagger \right) \right] |0_a\rangle \\
&= \sum_{l',m'} \left[a_j, 1 + \frac{1}{2} f_{l',m'} a_{l'}^\dagger a_{m'}^\dagger \right] \prod_{(l,m) \setminus (l',m')} \left(1 + \frac{1}{2} f_{l,m} a_l^\dagger a_m^\dagger \right) a_j |0_a\rangle \\
&= \sum_{l',m'} \frac{1}{2} f_{l',m'} \left(\delta_{j,l'} a_{m'}^\dagger - \delta_{j,m'} a_{l'}^\dagger \right) \prod_{(l,m) \setminus (l',m')} \left(1 + \frac{1}{2} f_{l,m} a_l^\dagger a_m^\dagger \right) a_j |0_a\rangle \\
&= \sum_{l',m'} \frac{1}{2} f_{l',m'} \left(\delta_{j,l'} a_{m'}^\dagger - \delta_{j,m'} a_{l'}^\dagger \right) \cdot \left(1 + \frac{1}{2} f_{l',m'} a_{l'}^\dagger a_{m'}^\dagger \right) \prod_{(l,m) \setminus (l',m')} \left(1 + \frac{1}{2} f_{l,m} a_l^\dagger a_m^\dagger \right) a_j |0_a\rangle \\
&= \sum_{l',m'} \frac{1}{2} f_{l',m'} \left(\delta_{j,l'} a_{m'}^\dagger - \delta_{j,m'} a_{l'}^\dagger \right) \prod_{l,m} \left(1 + \frac{1}{2} f_{l,m} a_l^\dagger a_m^\dagger \right) a_j |0_a\rangle \\
&= \left[\sum_{m'} \frac{1}{2} f_{j,m'} a_{m'}^\dagger - \sum_{l'} \frac{1}{2} f_{l',j} a_{l'}^\dagger \right] \prod_{l,m} \left(1 + \frac{1}{2} f_{l,m} a_l^\dagger a_m^\dagger \right) a_j |0_a\rangle \\
&= \left[\sum_{m'} \frac{1}{2} f_{j,m'} a_{m'}^\dagger + \sum_{l'} \frac{1}{2} f_{j,l'} a_{l'}^\dagger \right] \prod_{l,m} \left(1 + \frac{1}{2} f_{l,m} a_l^\dagger a_m^\dagger \right) a_j |0_a\rangle \\
&= \sum_k f_{j,k} a_k^\dagger \prod_{l,m} \left(1 + \frac{1}{2} f_{l,m} a_l^\dagger a_m^\dagger \right) a_j |0_a\rangle
\end{aligned}$$

于是 a_j 对 $|\Omega\rangle$ 的作用为

$$\begin{aligned}
a_j |\Omega\rangle &= \mathcal{N} a_j \prod_{l,m} \left(1 + \frac{1}{2} f_{l,m} a_l^\dagger a_m^\dagger \right) |0_a\rangle \\
&= \mathcal{N} \sum_k f_{j,k} a_k^\dagger \prod_{l,m} \left(1 + \frac{1}{2} f_{l,m} a_l^\dagger a_m^\dagger \right) a_j |0_a\rangle \\
&= \sum_k f_{j,k} a_k^\dagger |\Omega\rangle
\end{aligned} \tag{18}$$

基态由

$$\alpha_i |\Omega\rangle = 0 \tag{19}$$

确定, 也即

$$\sum_{j=1}^N \left(w_{ji}^* a_j + v_{ji}^* a_j^\dagger \right) |\Omega\rangle = 0 \tag{20}$$

把 $a_j |\Omega\rangle$ 代入:

$$\begin{aligned}
0 &= \sum_{j=1}^N \left(w_{ji}^* a_j + v_{ji}^* a_j^\dagger \right) |\Omega\rangle \\
&= \sum_{j=1}^N \left(w_{ji}^* \sum_k f_{j,k} a_k^\dagger + v_{ji}^* a_j^\dagger \right) |\Omega\rangle \\
&= \sum_{j=1}^N \left(w_{ji}^* \sum_k f_{j,k} a_k^\dagger + v_{ji}^* \sum_k \delta_{j,k} a_k^\dagger \right) |\Omega\rangle \\
&= \sum_{j=1}^N \left(\sum_k w_{ji}^* f_{j,k} a_k^\dagger + \sum_k v_{ji}^* \delta_{j,k} a_k^\dagger \right) |\Omega\rangle \\
&= \sum_{j=1}^N \sum_k \left(w_{ji}^* f_{j,k} a_k^\dagger + v_{ji}^* \delta_{j,k} a_k^\dagger \right) |\Omega\rangle \\
&= \sum_k \sum_{j=1}^N \left(w_{ji}^* f_{j,k} a_k^\dagger + v_{ji}^* \delta_{j,k} a_k^\dagger \right) |\Omega\rangle \\
&= \sum_k \left[\sum_{j=1}^N (w_{ji}^* f_{j,k} + v_{ji}^* \delta_{j,k}) \right] a_k^\dagger |\Omega\rangle
\end{aligned} \tag{21}$$

因此有

$$\sum_{j=1}^N (w_{ji}^* f_{j,k} + v_{ji}^* \delta_{j,k}) = 0, \quad \forall i, k \tag{22}$$

利用 $f_{j,k}$ 的反对称性有

$$\sum_{j=1}^N (-f_{k,j} w_{ji}^* + \delta_{k,j} v_{ji}^*) = 0, \quad \forall i, k \tag{23}$$

构造 \mathbf{f} 矩阵:

$$\mathbf{f} = \begin{pmatrix} f_{1,1} & f_{1,2} & \cdots \\ f_{2,1} & \ddots & \vdots \\ \vdots & \cdots & \ddots \end{pmatrix} \tag{24}$$

则化为

$$-(\mathbf{f}\mathbf{w}^*)_{k,i} + (\mathbf{I}\mathbf{v}^*)_{k,i} = 0, \quad \forall i, k \tag{25}$$

也即矩阵方程

$$\mathbf{f}\mathbf{w}^* = \mathbf{v}^* \tag{26}$$

于是

$$\mathbf{f} = \mathbf{v}^* (\mathbf{w}^*)^{-1} \tag{27}$$